FOL_Compactness/FOL_Semantics.thy
@@ -57,11 +57,11 @@ definition list_all :: \<open>('a \<Rightarrow> bool) \<Rightarrow> 'a list \<Ri
   [simp]: \<open>list_all P ls \<longleftrightarrow> (fold (\<lambda>l b. b \<and> P l) ls True)\<close>
 
 (*TERMSUBST_TERMVAL*)
-lemma term_subst_eval: "intrp_fn M = Fun \<Longrightarrow> t \<cdot> v = eval t M v"
+lemma term_subst_eval: \<open>intrp_fn M = Fun \<Longrightarrow> t \<cdot> v = eval t M v\<close>
   by (induction t) auto
 
 (*TERMVAL_TRIV*)
-lemma term_eval_triv[simp]: "intrp_fn M = Fun \<Longrightarrow> eval t M Var = t"
+lemma term_eval_triv[simp]: \<open>intrp_fn M = Fun \<Longrightarrow> eval t M Var = t\<close>
   by (metis subst_apply_term_empty term_subst_eval)
 
 lemma fold_bool_prop: \<open>(fold (\<lambda>l b. b \<and> P l) ls b) = (b \<and> (\<forall>l\<in>set ls. P l))\<close>
@@ -79,6 +79,23 @@ definition is_interpretation where
 lemma interpretation_sublanguage: \<open>funs2 \<subseteq> funs1 \<Longrightarrow> is_interpretation (funs1, pred1) \<M>
   \<Longrightarrow> is_interpretation (funs2, preds2) \<M>\<close>
   unfolding is_interpretation_def by auto
+
+(*INTERPRETATION_TERMVAL in HOL Light*)
+lemma interpretation_eval:
+  assumes \<M>: \<open>is_interpretation (functions_term t,any) \<M>\<close> and val: \<open>is_valuation \<M> \<beta>\<close>
+  shows \<open>\<lbrakk>t\<rbrakk>\<^bsup>\<M>,\<beta>\<^esup> \<in> dom \<M>\<close>
+  using \<M>
+proof (induction t)
+  case (Var x)
+  with val show ?case
+    by (simp add: is_valuation_def)
+next
+  case (Fun f ts)
+  then have \<open>\<lbrakk>t\<rbrakk>\<^bsup>\<M>,\<beta>\<^esup> \<in> dom \<M>\<close> if \<open>t \<in> set ts\<close> for t
+    by (meson interpretation_sublanguage supt.arg supt_imp_funas_term_subset that)
+  then show ?case
+    using Fun by (simp add: is_interpretation_def image_subsetI)
+qed
 
 (* Notation Warning: To prevent ambiguity with tuples, the comma is *bold* *)
 fun holds
@@ -279,7 +296,7 @@ next
   case (Forall x \<phi>)
   define \<sigma>' where "\<sigma>' = \<sigma>(x := Var x)"
   show ?case
-  proof (cases "\<exists> y. y \<in> FV (\<^bold>\<forall> x\<^bold>. \<phi>) \<and> x \<in> FVT (\<sigma>' y)")
+  proof (cases \<open>\<exists> y. y \<in> FV (\<^bold>\<forall> x\<^bold>. \<phi>) \<and> x \<in> FVT (\<sigma>' y)\<close>)
     case False
     then have \<open>(\<^bold>\<forall>x\<^bold>. \<phi>) \<cdot>\<^sub>f\<^sub>m \<sigma> = \<^bold>\<forall>x\<^bold>. (\<phi> \<cdot>\<^sub>f\<^sub>m \<sigma>')\<close>
       using formsubst_def_switch \<sigma>'_def by fastforce
@@ -424,7 +441,7 @@ next
   qed
 qed auto
 
-definition satisfies :: "'m intrp \<Rightarrow> form set \<Rightarrow> bool" where
+definition satisfies :: \<open>'m intrp \<Rightarrow> form set \<Rightarrow> bool\<close> where
   \<open>satisfies \<M> S \<equiv> (\<forall>\<beta> \<phi>. is_valuation \<M> \<beta> \<longrightarrow> \<phi> \<in> S \<longrightarrow> \<M>\<^bold>,\<beta> \<Turnstile> \<phi>)\<close>
 
 lemma satisfies_iff_satisfies_sing: \<open>satisfies M S \<longleftrightarrow> (\<forall>\<phi>\<in>S. satisfies M {\<phi>})\<close>
